proof/spec/KyberLib.ec
@@ -1,0 +1,515 @@
+require import AllCore IntDiv FloorCeil StdOrder RealExp List.
+require import ZModP Ring.
+require import Distr DList DistrExtra DMap DInterval.
+require import PKE_Ext.
+from Jasmin require import JWord JUtils.
+require import Array25 Array32 Array34 Array64 Array128 Array168 Array256 Array384.
+require import Array768 Array960 Array1024 Array1088 Array1184 Array1152.
+require  PRF.
+
+
+(*---*) import RField RealOrder IntOrder IntID.
+
+(**************************************************)
+(* Aux stuff needed for compression/decompression *)
+(**************************************************)
+(**************************************************)
+(* MOVE THIS TO ECLIB!!!                          *)
+(**************************************************)
+
+lemma floorDz (x:int) y:
+ floor (x%r + y) = x + floor y.
+proof.
+rewrite (floorE (x+floor y)) //.
+smt(floor_bound).
+qed.
+
+lemma nosmt le_floorE n x:
+ (n <= floor x) = (n%r <= x)
+by smt(floor_bound).
+
+lemma nosmt floor_ltE x n:
+ (floor x < n) = (x < n%r)
+by smt(floor_bound).
+
+lemma divz_floor (x y: int):
+ 0 < y =>
+ x %/ y = floor (x%r / y%r).
+proof.
+move=> gt0.
+have ->: x%r / y%r = (x %/ y)%r + (x %% y)%r / y%r.
+ by rewrite {1}(divz_eq x y); field; smt(). 
+rewrite floorDz.
+have ?: 0%r <= (x %% y)%r / y%r < 1%r. 
+  rewrite ltr_pdivr_mulr /=; 1: smt().
+  split; smt(le_fromint RealOrder.divr_ge0).
+by smt(floor_bound).
+qed.
+
+lemma modz_floor (x y: int):
+ 0 < y =>
+ x %% y = x - y * floor (x%r / y%r).
+proof.
+move=> gt0.
+rewrite -divz_floor //; smt(divz_eq).
+qed.
+
+
+op frac (x: real) = x - (floor x)%r.
+
+lemma frac_bound x: 0%r <= frac x < 1%r
+by smt(floor_bound).
+
+lemma fracDz x n: frac (n%r + x) = frac x
+by smt(floorDz).
+
+lemma floor_frac_eq x: x = (floor x)%r + frac x
+by smt().
+
+lemma frac0_dvdz (m n: int):
+ 0 < n =>
+ frac (m%r / n%r) = 0%r <=> n %| m.
+proof. 
+move=> ygt0; rewrite dvdzE modz_floor // /frac. 
+split; 1: by smt().
+rewrite -divz_floor //. 
+move => H.
+have ->  /=: m = n*(m %/ n); 1: by smt().
+by ring; smt().
+qed.
+
+lemma from_int_frac n: frac n%r = 0%r
+by smt(from_int_floor).
+
+lemma frac_halfP x:
+ frac x = inv 2%r => frac (2%r*x) = 0%r.
+proof.
+move => E; rewrite floor_frac_eq mulrDr.
+by rewrite -fromintM fracDz E divrr // from_int_frac.
+qed.
+
+lemma frac_halfN x:
+ frac (2%r*x) <> 0%r => frac x <> inv 2%r
+by smt(frac_halfP).
+
+lemma frac_div_eq0 (m n: int):
+ 0 < n =>
+ frac (m%r / n%r) = 0%r
+ <=> n %| m.
+proof.
+move=> gt0.
+split => H.
+ have E: m%r / n%r = (m %/ n)%r.
+  rewrite (floor_frac_eq (m%r / n%r)) H/= divz_floor /#.
+ have : m%r = (m %/ n)%r * n%r + (m %% n)%r by smt(divz_eq).
+ by rewrite -E dvdzE /#.
+have : m%r = (m %/ n)%r * n%r + (m %% n)%r by smt(divz_eq).
+rewrite H /= => ->.
+rewrite /frac; smt(floorE).
+qed.
+
+lemma frac_inv_gt1 x: 1%r < x => frac (inv x) = inv x.
+proof. by move=> H; rewrite /frac; smt(floor_bound). qed.
+
+
+op round(x : real) : int = floor (x + inv 2%r).
+
+lemma round_mono (x y: real):
+ x <= y => round x <= round y
+by smt(floor_mono).
+
+lemma round_divz x y:
+ 0 < y => 
+ round (x%r / y%r) = (2*x+y) %/ (2*y).
+proof.
+move=> H; rewrite /round.
+have ->: x%r / y%r + inv 2%r = (2* x + y)%r / (2*y)%r.
+ rewrite fromintD !fromintM; field; smt().
+by rewrite divz_floor /#.
+qed.
+
+require import Real RealExp StdRing.
+lemma roundDz (x:int) y:
+ round (x%r + y) = x + round y.
+proof. by rewrite /round -addrA floorDz. qed.
+
+lemma from_int_round n: round n%r = n.
+proof. by rewrite /round (floorE n) /#. qed. 
+
+lemma round_ge0 x: 0%r <= x => 0 <= round x
+by smt(floor_bound).
+
+lemma round_bound x:
+ x - inv(2%r) < (round x)%r <= x + inv(2%r)
+by smt(floor_bound).
+
+lemma nosmt le_roundE n x:
+ (n <= round x) = (n%r <= x + inv 2%r)
+by smt(le_floorE).
+
+lemma nosmt round_ltE x n:
+ (round x < n) = (x + inv 2%r < n%r)
+by smt(floor_ltE).
+
+
+lemma nosmt roundN x:
+ frac x <> inv 2%r => round (-x) = -round x.
+proof.
+move => H.
+pose nn := round (-x).
+have <-:= floorE (round x) (-nn%r+inv 2%r).
+ have [??]:= round_bound (-x).
+ have ?: -nn%r < x + inv 2%r by smt().
+ have ?: x - inv 2%r <= -nn%r by smt().
+ have ?: x - inv 2%r < -nn%r.
+  have /#: x - inv 2%r <> -nn%r.
+  apply (contra _ (frac x = inv 2%r)).
+  move => E.
+  have ->: x = (-nn)%r + inv 2%r by smt().
+   by rewrite fracDz frac_inv_gt1 /#.
+  smt().
+ smt(round_bound). 
+by rewrite -fromintN floorDz; smt(floorE).
+qed.
+
+
+lemma normP (a epsilon: int):
+ `| a | <= epsilon <=> -epsilon <= a <= epsilon
+by smt().
+
+
+
+
+lemma flatten_rcons ['a] (l: 'a list list) x:
+ flatten (rcons l x) = flatten l ++ x.
+proof.
+elim: l => /=.
+ by rewrite flatten_cons !flatten_nil cats0.
+by move=> y l IH; rewrite !flatten_cons IH catA.
+qed.
+
+
+
+
+
+lemma dlist_mul ['a] (d: 'a distr) (k n: int):
+ 0 <= k => 0 <= n =>
+ dlist d (k*n) = dmap (dlist (dlist d k) n) flatten.
+proof.
+move=> Hk; elim/natind: n.
+ move=> n Hn0 Hn; have ->/=: n=0 by smt().
+ by rewrite !dlist0 // dmap_dunit flatten_nil.
+move=> n Hn IH _; have->: k*(n+1) = k + k*n by ring.
+rewrite dlist_add // 1:/# dlistS //.
+rewrite dmap_comp IH // dmap_dprodR dmap_comp /(\o) /=.
+apply eq_dmap; move => [xh xt] /=.
+by rewrite flatten_cons.
+qed.
+
+
+
+(* JASMIN ECLIB *)
+
+(* JWord.ec *)
+import BitEncoding BitChunking BS2Int.
+
+lemma W8all_words_uniq: uniq W8.all_words.
+proof.
+rewrite /W8.all_words map_inj_in_uniq.
+ move=> x y; rewrite !mem_iota => /= ?? H.
+ have: x %% W8.modulus = y %% W8.modulus.
+  by rewrite -!W8.of_uintK H.
+ by rewrite !modz_small /#.
+by apply iota_uniq.
+qed.
+
+lemma dword1E w:
+ mu1 W8.dword w = inv (W8.modulus%r).
+proof.
+have ?:= W8all_words_uniq.
+rewrite /W8.dword /duniform undup_id //.
+rewrite MRat.dratE count_uniq_mem //.
+rewrite W8.all_wordsP b2i1.
+rewrite /W8.all_words size_map size_iota /=.
+by rewrite ler_maxr.
+qed.
+
+lemma dword1E_bits w:
+ mu1 (dmap (dlist {0,1} W8.size) W8.bits2w) w = inv (W8.modulus)%r.
+proof.
+rewrite dmap1E /(\o) /=.
+rewrite (mu_eq_support _ _ (pred1 (w2bits w))).
+ move=> l; rewrite supp_dlist //=; move=> [E _].
+ rewrite /pred1.
+ apply eqboolP; split => H.
+  by rewrite -H W8.bits2wK.
+ by rewrite H W8.w2bitsK.
+rewrite dlist1E // W8.size_w2bits /=.
+rewrite (StdBigop.Bigreal.BRM.eq_bigr _ _ (fun _=>inv 2%r)).
+ by move=> i _ /=; rewrite DBool.dbool1E /#. 
+rewrite StdBigop.Bigreal.mulr_const.
+rewrite W8.size_w2bits.
+by rewrite RealOrder.Domain.exprVn // fromintXn //.
+qed.
+
+lemma dword_bits:
+ W8.dword = dmap (dlist {0,1} 8) W8.bits2w.
+proof.
+apply eq_distr => w.
+by rewrite dword1E dword1E_bits.
+qed.
+
+require import DInterval.
+lemma dword_ibits:
+ W8.dword = dmap (dbits 8) W8.of_int.
+proof.
+apply eq_distr => w.
+rewrite dword1E dmap1E /(\o) /=.
+rewrite (mu_eq_support _ _ (pred1 (to_uint w))).
+ move=> x; rewrite supp_dinter //= => E.
+ rewrite /pred1.
+ apply eqboolP; split => H.
+  by rewrite -H W8.of_uintK modz_small /#.
+ by rewrite H W8.to_uintK.
+rewrite dinter1E.
+rewrite (_: 0 <= to_uint w <= 255) //=.
+by move: (W8.to_uint_cmp w) => /= /#.
+qed.
+
+(* JArray.ec *)
+(* useful for loop-invariants: relating arrays and lists... *)
+op a256l ['a] (a:'a Array256.t) (l:'a list) k: bool = size l = k /\ 
+ forall i, 0 <= i < k => a.[i] = nth witness l i.
+
+lemma a256l_rcons ['a] a l (x:'a) k:
+ 0 <= k < 256 =>
+ a256l a l k => 
+ a256l a.[k <- x] (rcons l x) (k+1).
+proof.
+move=> Hk; rewrite /a256l; move=> [Hsize H].
+rewrite size_rcons Hsize; split => // i Hi.
+rewrite get_setE // nth_rcons Hsize.
+case: (i=k) => E.
+ by rewrite E.
+by rewrite H /#.
+qed.
+
+lemma a256l_of_list ['a] a (l: 'a list):
+ a256l a l 256 =>
+ a = Array256.of_list witness l.
+proof.
+move=> [Hsize H].
+apply Array256.ext_eq => i Hi.
+by rewrite H // get_of_list //.
+qed.
+
+
+
+op darray32 ['a] (d: 'a distr): ('a Array32.t) distr =
+ dmap (dlist d 32) (Array32.of_list witness).
+
+lemma darray32_ll ['a] (d: 'a distr):
+ is_lossless d => is_lossless (darray32 d).
+proof.  by rewrite /darray32 => ?; apply dmap_ll; apply dlist_ll. qed.
+
+(*
+module Sample_darray32 = {
+ proc sample(d: W8.t distr) = {
+  var w;
+  w <$ darray32 d;
+  return w;
+ }
+ proc sampleL(d: W8.t distr) = {
+  var l;
+   l <$ dlist d 32;
+   return Array32.of_list witness l;
+  }
+}.
+*)
+
+clone DMapSampling as MSa32 with
+ type t1 <- W8.t list,
+ type t2 <- W8.t Array32.t.
+
+clone DMapSampling as MSa64 with
+ type t1 <- W8.t list,
+ type t2 <- W8.t Array64.t.
+
+clone DProd.ProdSampling as PSlw with
+ type t1 <- W8.t list,
+ type t2 <- W8.t list.
+
+clone DMapSampling as MSll with
+ type t1 <- W8.t list * W8.t list,
+ type t2 <- W8.t list.
+
+op darray64 ['a] (d: 'a distr): ('a Array64.t) distr =
+ dmap (dlist d 64) (Array64.of_list witness).
+
+lemma darray64_ll ['a] (d: 'a distr):
+ is_lossless d => is_lossless (darray64 d).
+proof.  by rewrite /darray64 => ?; apply dmap_ll; apply dlist_ll. qed.
+
+module Sample_64_2x32 = {
+ proc sample() = {
+  var w;
+  w <$ darray64 W8.dword;
+  return w;
+ }
+ proc sample2() = {
+  var w1, w2;
+  w1 <$ darray32 W8.dword;
+  w2 <$ darray32 W8.dword;
+  return (w1, w2);
+ }
+}.
+
+lemma aux_64_32x32 (l1 l2: W8.t list) a:
+ size l1 = 32 => 
+ a = Array64.of_list witness (l1++l2) =>
+ Array32.init (fun i => a.[i]) = Array32.of_list witness l1 /\
+ Array32.init (fun i => a.[32+i]) = Array32.of_list witness l2.
+proof.
+move=> Hl1 ->.
+have X: forall (l: W8.t list), Array32.of_list witness l = Array32.init (fun i => nth witness l i).
+ move=> l; rewrite tP => i Hi.
+ by rewrite get_of_list // initE Hi.
+rewrite !X !tP.
+split => i Hi;  rewrite !initE !Hi /= get_of_list 1:/# nth_cat.
+ by have ->:i < size l1 by smt().
+by have ->/#:! 32+i < size l1 by smt().
+qed.
+
+equiv sample_64_2x32_eq:
+ Sample_64_2x32.sample ~ Sample_64_2x32.sample2:
+ true ==> res{2}.`1 = Array32.init (fun i=>res{1}.[i]) /\ res{2}.`2 = Array32.init (fun i=>res{1}.[i+32]).
+proof.
+proc.
+transitivity {1} { w <@ MSa64.S.sample(dlist W8.dword 64, Array64.of_list witness); }
+ ( true ==> ={w} )
+ ( true ==> w1{2} = Array32.init (fun (i : int) => w{1}.[i]) /\
+            w2{2} = Array32.init (fun (i : int) => w{1}.[i+32]) ) => //=.
+- by inline*; auto.
+transitivity {1} { w <@ MSa64.S.map(dlist W8.dword 64, Array64.of_list witness); }
+ ( true ==> ={w} )
+ ( true ==> w1{2} = Array32.init (fun (i : int) => w{1}.[i]) /\
+            w2{2} = Array32.init (fun (i : int) => w{1}.[i+32]) ) => //=.
+- by call MSa64.sample.
+transitivity {2} 
+ { w1 <@ MSa32.S.sample(dlist W8.dword 32, Array32.of_list witness); 
+   w2 <@ MSa32.S.sample(dlist W8.dword 32, Array32.of_list witness); }
+ ( true ==> w1{2} = Array32.init (fun (i : int) => w{1}.[i]) /\
+            w2{2} = Array32.init (fun (i : int) => w{1}.[i+32]) )
+ ( true ==> ={w1, w2} ) => //=; last first.
+- by inline*; auto.
+transitivity {2} 
+ { w1 <@ MSa32.S.map(dlist W8.dword 32, Array32.of_list witness); 
+   w2 <@ MSa32.S.map(dlist W8.dword 32, Array32.of_list witness); }
+ ( true ==> w1{2} = Array32.init (fun (i : int) => w{1}.[i]) /\
+            w2{2} = Array32.init (fun (i : int) => w{1}.[i+32]) )
+ ( true ==> ={w1, w2} ) => //=; last first.
+- by symmetry; do 2! call MSa32.sample.
+inline*.
+swap{1} 2 1; swap {2} 6 1; swap {2} 2 1; swap {2} [3..4] 2; wp.
+conseq (_:_ ==> size r1{2}=32 /\ r1{1}=r1{2}++r10{2}).
+ move=> /> l1 l2 H.
+ move: (aux_64_32x32 l1 l2 (of_list witness (l1 ++ l2))%Array64 H).
+ by move => [<- <-] /#.
+transitivity {2} { (r1,r10) <@ PSlw.S.sample2(dlist W8.dword 32, dlist W8.dword 32); }
+ ( true ==> size r1{2} = 32 /\  r1{1} = r1{2} ++ r10{2} )
+ ( true ==> ={r1, r10} ) => //=; last by inline*; auto.
+transitivity {2} { (r1,r10) <@ PSlw.S.sample(dlist W8.dword 32, dlist W8.dword 32); }
+ ( true ==> size r1{2} = 32 /\  r1{1} = r1{2} ++ r10{2} )
+ ( true ==> ={r1, r10} ) => //=; last by call PSlw.sample_sample2.
+inline*; wp; simplify.
+transitivity {1} { r1 <@ MSll.S.sample(dlist W8.dword 32 `*` dlist W8.dword 32, fun ll:_*_=>ll.`1 ++ ll.`2); }
+ ( true ==> ={r1} )
+ ( true ==> size r{2}.`1 = 32 /\ r1{1} = r{2}.`1 ++ r{2}.`2 ) => //=.
+- by inline*; auto => />; rewrite (_:64=32+32) 1:/# dlist_add /#.
+transitivity {1} { r1 <@ MSll.S.map(dlist W8.dword 32 `*` dlist W8.dword 32, fun ll:_*_=>ll.`1 ++ ll.`2); }
+ ( true ==> ={r1} )
+ ( true ==> size r{2}.`1 = 32 /\ r1{1} = r{2}.`1 ++ r{2}.`2 ) => //=; first by call MSll.sample.
+by inline*; auto => /> ll; rewrite supp_dprod supp_dlist /#.
+qed.
+
+op darray128 ['a] (d: 'a distr): ('a Array128.t) distr =
+ dmap (dlist d 128) (Array128.of_list witness).
+
+(* proof-templates (to be included in the DArray theory...) *)
+lemma darray128_ll ['a] (d: 'a distr):
+ is_lossless d => is_lossless (darray128 d).
+proof. by rewrite /darray128 => ?; apply dmap_ll; apply dlist_ll. qed.
+
+lemma supp_darray128 ['a] (d: 'a distr) a:
+ a \in darray128 d <=> all (support d) (Array128.to_list a).
+proof.
+rewrite /darray128 supp_dmap; split.
+ move=> [x]; rewrite supp_dlist // => /> *.
+ by rewrite Array128.of_listK // /#.
+move=> H; exists (to_list a); rewrite supp_dlist // H Array128.size_to_list /=.
+by rewrite Array128.to_listK.
+qed.
+
+lemma darray128_uni ['a] (d: 'a distr):
+ is_uniform d => is_uniform (darray128 d).
+proof.
+rewrite /darray128=> ?; apply dmap_uni_in_inj.
+ move=> x y; rewrite !supp_dlist //; move => [? _] [? _] H.
+ by rewrite -(Array128.of_listK witness x) // H of_listK.
+by apply dlist_uni.
+qed.
+
+lemma darray128_fu ['a] (d: 'a distr):
+ is_full d => is_full (darray128 d).
+proof.
+rewrite /darray128 => H; apply dmap_fu_in.
+move=> x; exists (to_list x); rewrite to_listK supp_dlist //=.
+rewrite Array128.size_to_list /= allP => *.
+by apply H.
+qed.
+
+
+op darray168 ['a] (d: 'a distr): ('a Array168.t) distr =
+ dmap (dlist d 168) (Array168.of_list witness).
+
+(* ... *)
+
+
+op darray256 ['a] (d: 'a distr): ('a Array256.t) distr =
+ dmap (dlist d 256) (Array256.of_list witness).
+
+lemma darray256_ll ['a] (d: 'a distr):
+ is_lossless d => is_lossless (darray256 d).
+proof.  by rewrite /darray256 => ?; apply dmap_ll; apply dlist_ll. qed.
+
+lemma supp_darray256 ['a] (d: 'a distr) a:
+ a \in darray256 d <=> all (support d) (Array256.to_list a).
+proof.
+rewrite /darray256 supp_dmap; split.
+ move=> [x]; rewrite supp_dlist // => /> *.
+ by rewrite Array256.of_listK // /#.
+move=> H; exists (to_list a); rewrite supp_dlist // H Array256.size_to_list /=.
+by rewrite Array256.to_listK.
+qed.
+
+lemma darray256_uni ['a] (d: 'a distr):
+ is_uniform d => is_uniform (darray256 d).
+proof.
+rewrite /darray256=> ?; apply dmap_uni_in_inj.
+ move=> x y; rewrite !supp_dlist //; move => [? _] [? _] H.
+ by rewrite -(Array256.of_listK witness x) // H of_listK.
+by apply dlist_uni.
+qed.
+
+lemma darray256_fu ['a] (d: 'a distr):
+ is_full d => is_full (darray256 d).
+proof.
+rewrite /darray256 => H; apply dmap_fu_in.
+move=> x; exists (to_list x); rewrite to_listK supp_dlist //=.
+rewrite Array256.size_to_list /= allP => *.
+by apply H.
+qed.
+
+
+
+
